Express cache as mem
Probably want to have linearizability for the cache as well, in order to
accurately express how the (single) disk and (linearizable) virtual disk
are related.

src/MemCache2.v
@@ -1,5 +1,6 @@
 Require Import EventCSL.
 Require Import EventCSLauto.
+Require Import FunctionalExtensionality.
 Require Import Preservation.
 Require Import FMapAVL.
 Require Import FMapFacts.
@@ -19,34 +20,42 @@ Section MemCache.
 
 Inductive cache_entry :=
   | Clean (v:valu)
-  | Dirty (v:valu)
-  | Missing.
+  | Dirty (v:valu).
 
 Definition BlockCache : Type := Map.t cache_entry.
+Definition BlockFun := @mem addr _ (const cache_entry).
 
-Definition cache_get c a :=
-  match Map.find a c with
-  | Some v => v
-  | None => Missing
-  end.
+Definition cache_get (c: BlockCache) (a: addr) :=
+  Map.find a c.
 
-Definition cache_add c a v :=
+Definition cache_add (c: BlockCache) (a: addr) v :=
   Map.add a (Clean v) c.
 
-Definition cache_dirty c a v :=
+Definition cache_dirty (c: BlockCache) (a: addr) v :=
   Map.add a (Dirty v) c.
 
 End MemCache.
 
-Definition cache_rep (c: BlockCache) (d: DISK) : DISK_PRED :=
+Definition cache_fun_rep (c: BlockCache) (cf: BlockFun) : Prop :=
+  cf = cache_get c.
+
+Lemma cache_fun_rep_ext : forall c cf,
+    (forall a, cf a = cache_get c a) ->
+    cache_fun_rep c cf.
+Proof.
+  intros.
+  unfold cache_fun_rep; extensionality a; eauto.
+Qed.
+
+Definition cache_rep (c: BlockFun) (d: DISK) : DISK_PRED :=
   fun vd =>
     forall a,
-    match cache_get c a with
-    | Clean v => exists reader,
+    match c a with
+    | Some (Clean v) => exists reader,
       d a = Some (v, reader) /\
       vd a = Some (v, reader)
-    | Dirty v => exists v0 reader,
+    | Some (Dirty v) => exists v0 reader,
       d a = Some (v0, reader) /\
       vd a = Some (v, reader)
-    | Invalid => d a = vd a
+    | None => d a = vd a
     end.
